entropy.v
@@ -1,0 +1,20 @@
+Require Import List ZArith.
+
+Require Import basic_types.
+
+Inductive bitstream_position :=
+  bitstream_postion_intro : Z -> Z -> bitstream_position.
+
+Inductive bitstream_at_relation :
+    bitstream -> bitstream_position -> bit -> Prop :=
+  bitstream_at_relation_intro :
+    forall bs byte_index bit_index value,
+      False(* TODO *) ->
+      bitstream_at_relation bs (bitstream_postion_intro byte_index bit_index)
+        value.
+
+Inductive read_bit_relation :
+    bitstream -> bitstream_position -> bit -> bitstream_position -> Prop :=
+  | read_bit_relation_intro :
+    forall bs bp0 b bp1,
+      
