state.v
@@ -1,0 +1,396 @@
+Require Import ZArith.
+Require Import String.
+Require Import Ascii.
+Require Import Relations.
+Require Import OrderedType.
+Require Import OrderedTypeEx.
+
+Definition lt_not_eq_prop {X : Type} (eq lt : X -> X -> Prop) : Prop :=
+  forall (x y : X),
+    lt x y -> ~(eq x y).
+
+Module list_as_MiniOT (X : OrderedType) <: MiniOrderedType.
+
+  Definition t := list X.t.
+
+  Inductive eq_dummy : t -> t -> Prop :=
+    | eq_nil :
+      eq_dummy nil nil
+    | eq_more :
+      forall h0 h1 t0 t1,
+      X.eq h0 h1 -> eq_dummy t0 t1 -> eq_dummy (h0 :: t0) (h1 :: t1).
+
+  Definition eq := eq_dummy.
+
+  Inductive lt_dummy : t -> t -> Prop :=
+    | lt_nil :
+      forall h t,
+        lt_dummy nil (h :: t)
+    | lt_h :
+      forall h0 h1 t0 t1,
+        X.lt h0 h1 -> lt_dummy (h0 :: t0) (h1 :: t1)
+    | lt_t :
+      forall h0 h1 t0 t1,
+        X.eq h0 h1 -> lt_dummy t0 t1 -> lt_dummy (h0 :: t0) (h1 :: t1).
+
+  Definition lt := lt_dummy.
+
+  Theorem eq_refl : reflexive t eq.
+  Proof.
+    intros l.
+    induction l.
+    - apply eq_nil.
+    - apply eq_more.
+      + apply X.eq_refl.
+      + apply IHl.
+  Qed.
+
+  Theorem eq_sym : symmetric t eq.
+  Proof.
+    intros l.
+    induction l.
+    - intros x Hx.
+      inversion Hx.
+      apply eq_refl.
+    - intros y Hy.
+      destruct y.
+      + inversion Hy.
+      + inversion Hy;
+          subst.
+        apply eq_more.
+        * apply X.eq_sym.
+          auto.
+        * apply IHl.
+          auto.
+  Qed.
+
+  Definition eq_trans : transitive t eq.
+  Proof.
+    intros x y z H_xy.
+    generalize z.
+    induction H_xy.
+    - intros z0 H_yz.
+      auto.
+    - intros z0 H_yz.
+      inversion H_yz;
+        subst.
+      apply eq_more.
+      + apply X.eq_trans with h1;
+          auto.
+      + apply IHH_xy.
+        auto.
+  Qed.
+
+  Theorem lt_trans : transitive t lt.
+  Proof.
+    intros x y z H_xy.
+    generalize z.
+    induction H_xy.
+    - intros z0 H_yz.
+      inversion H_yz;
+        apply lt_nil.
+    - intros z0 H_yz.
+      inversion H_yz;
+        subst.
+      + apply lt_h.
+        apply X.lt_trans with h1;
+          auto.
+      + apply lt_h.
+        (* TODO: replace this part with some ready proof on X *)
+        destruct (X.compare h0 h3).
+        * auto.
+        * exfalso.
+          apply X.lt_not_eq with h0 h1; 
+            auto.
+          apply X.eq_trans with h3;
+            auto.
+        * exfalso.
+          apply X.lt_not_eq with h3 h1;
+            auto.
+          apply X.lt_trans with h0;
+            auto.
+    - intros z0 H_yz.
+      inversion H_yz;
+        subst.
+      + apply lt_h.
+        destruct (X.compare h0 h3).
+        * auto.
+        * exfalso.
+          apply X.lt_not_eq with h1 h3;
+            auto.
+          apply X.eq_trans with h0;
+            auto.
+        * exfalso.
+          apply X.lt_not_eq with h1 h0;
+            auto.
+          apply X.lt_trans with h3;
+            auto.
+      + apply lt_t.
+        * apply X.eq_trans with h1;
+            auto.
+        * apply IHH_xy.
+          auto.
+  Qed.
+
+  Theorem lt_not_eq : lt_not_eq_prop eq lt.
+  Proof.
+    intros x y Hlt Heq.
+    induction Hlt;
+      subst.
+    - inversion Heq.
+    - inversion Heq;
+        subst.
+      apply X.lt_not_eq with h0 h1;
+        auto.
+    - inversion Heq;
+        subst.
+      auto.
+  Qed.
+
+  Definition compare l0 l1 : Compare lt eq l0 l1.
+  Proof.
+    generalize l1.
+    induction l0 as [| h0 t0].
+    - intros l2.
+      destruct l2 as [| h1 t1].
+      + apply EQ.
+        apply eq_refl.
+      + apply LT.
+        apply lt_nil.
+    - intros l2.
+      destruct l2 as [| h1 t1].
+      + apply GT.
+        apply lt_nil.
+      + destruct (X.compare h0 h1).
+        * apply LT.
+          apply lt_h.
+          auto.
+        * destruct IHt0 with t1.
+          { apply LT.
+            apply lt_t;
+              auto. }
+          { apply EQ.
+            apply eq_more;
+              auto. }
+          { apply GT.
+            apply lt_t;
+              auto. }
+        * apply GT.
+          apply lt_h.
+          auto.
+  Qed.
+End list_as_MiniOT.
+
+Module list_as_OT (X : OrderedType) <: OrderedType.
+  Module list_as_MiniOT_X := list_as_MiniOT X.
+  Include MOT_to_OT list_as_MiniOT_X.
+End list_as_OT.
+
+(* An expression might evaluate to reference to single variable or array element.
+   Reference to single variable is label with empty subscrtip list. *)
+Inductive reference :=
+  | ref_variable : string -> list Z -> reference.
+
+Definition lt_ascii (c0 c1 : ascii) : Prop :=
+  N.lt (N_of_ascii c0) (N_of_ascii c1).
+
+Lemma lt_ascii_trans :
+  transitive ascii lt_ascii.
+Proof.
+  intros x y z lt_xy lt_yz.
+  apply N.lt_trans with (m := N_of_ascii y); auto.
+Qed.
+
+Lemma lt_ascii_not_eq :
+  lt_not_eq_prop eq lt_ascii.
+Proof.
+  intros x y H Hinv.
+  subst.
+  unfold lt_ascii in H.
+  apply N.lt_irrefl with (N_of_ascii y).
+  auto.
+Qed.
+
+Definition compare_ascii (c0 c1 : ascii) : Compare lt_ascii (@eq ascii) c0 c1.
+Proof.
+  destruct (N_as_OT.compare (N_of_ascii c0) (N_of_ascii c1)).
+  - apply LT.
+    apply l.
+  - apply EQ.
+    unfold N_as_OT.eq in e.
+    rewrite <- ascii_N_embedding.
+    rewrite <- e.
+    rewrite ascii_N_embedding.
+    reflexivity.
+  - apply GT.
+    apply l.
+Defined.
+
+Inductive lt_string : string -> string -> Prop :=
+  | lt_string_empty :
+    forall c s, lt_string EmptyString (String c s)
+  | lt_string_x :
+    forall c0 c1 s0 s1,
+      lt_ascii c0 c1 -> lt_string (String c0 s0) (String c1 s1)
+  | lt_string_l :
+    forall c s0 s1,
+      lt_string s0 s1 -> lt_string (String c s0) (String c s1).
+
+Lemma lt_string_trans :
+  transitive string lt_string.
+Proof.
+  intros x y z H_xy.
+  generalize z.
+  induction H_xy.
+  - intros z0 H_yz.
+    inversion H_yz;
+      apply lt_string_empty.
+  - intros z0 H_yz.
+    inversion H_yz; subst.
+    + apply lt_string_x.
+      apply lt_ascii_trans with c1;
+        auto.
+    + apply lt_string_x; auto.
+  - intros z0 H_yz.
+    inversion H_yz; subst.
+    + apply lt_string_x;
+        auto.
+    + apply lt_string_l.
+      apply IHH_xy.
+      auto.
+Qed.
+
+Lemma lt_string_not_eq :
+  lt_not_eq_prop eq lt_string.
+Proof.
+  intros x y H.
+  induction H.
+  - intros Hinv.
+    inversion Hinv.
+  - intros Hinv.
+    inversion Hinv; subst.
+    apply lt_ascii_not_eq in H.
+    apply H.
+    reflexivity.
+  - intros Hinv.
+    inversion Hinv; subst.
+    apply IHlt_string.
+    reflexivity.
+Qed.
+
+Fixpoint compare_string (l0 l1 : string) :
+  Compare lt_string (@eq string) l0 l1.
+Proof.
+  destruct l0 as [| h0 t0].
+  - destruct l1 as [| h1 t1].
+    + apply EQ.
+      reflexivity.
+    + apply LT.
+      apply lt_string_empty.
+  - destruct l1 as [| h1 t1].
+    + apply GT.
+      apply lt_string_empty.
+    + destruct (compare_ascii h0 h1).
+      * apply LT.
+        apply lt_string_x.
+        auto.
+      * subst.
+        destruct (compare_string t0 t1).
+        { apply LT.
+          apply lt_string_l.
+          auto. }
+        { apply EQ.
+          subst.
+          reflexivity. }
+        { apply GT.
+          apply lt_string_l.
+          auto. }
+      * apply GT.
+        apply lt_string_x.
+        auto.
+Defined.
+
+Module list_Z_as_OT := list_as_OT Z_as_OT.
+
+Inductive lt_reference : reference -> reference -> Prop :=
+  | lt_reference_string :
+    forall s0 s1 l0 l1,
+      lt_string s0 s1 -> lt_reference (ref_variable s0 l0) (ref_variable s1 l1)
+  | lt_reference_list :
+    forall s l0 l1,
+      list_Z_as_OT.lt l0 l1 -> lt_reference (ref_variable s l0) (ref_variable s l1).
+
+Theorem lt_reference_trans :
+  transitive reference lt_reference.
+Proof.
+  intros x y z H_xy H_yz.
+  destruct H_xy as [xs ys xl yl H_xy | s xl yl H_xy].
+  - destruct z as [zs zl].
+    apply lt_reference_string.
+    inversion H_yz as [ys0 zs0 yl0 zl0 H_yz0 | s2 yl0 zl0 H_yz0]; subst.
+    + apply lt_string_trans with ys;
+        auto.
+    + auto.
+  - inversion H_yz as [ys zs yl0 zl H_yz0 | s2 yl0 zl H_yz0]; subst.
+    + apply lt_reference_string.
+      auto.
+    + apply lt_reference_list.
+      apply list_Z_as_OT.lt_trans with yl;
+        auto.
+Qed.
+
+Theorem lt_reference_not_eq :
+  lt_not_eq_prop eq lt_reference.
+Proof.
+  unfold lt_not_eq_prop.
+  intros.
+  inversion H; subst.
+  - intros Hinv.
+    inversion Hinv; subst.
+    apply lt_string_not_eq in H0.
+    auto.
+  - intros Hinv.
+    inversion Hinv; subst.
+    apply list_Z_as_OT.lt_not_eq in H0.
+    * apply H0.
+      apply list_Z_as_OT.eq_refl.
+Qed.
+
+Module ascii_as_OT <: UsualOrderedType.
+  Definition t := ascii.
+  Definition eq := @eq t.
+  Definition lt := lt_ascii.
+  Definition eq_refl := @eq_refl ascii.
+  Definition eq_sym := @eq_sym ascii.
+  Definition eq_trans := @eq_trans ascii.
+  Definition lt_trans := lt_ascii_trans.
+  Definition lt_not_eq := lt_ascii_not_eq.
+  Definition compare x y := compare_ascii x y.
+  Definition eq_dec := ascii_dec.
+End ascii_as_OT.
+
+Module string_as_OT <: UsualOrderedType.
+  Definition t := string.
+  Definition eq := @eq string.
+  Definition lt := lt_string.
+  Definition eq_refl := @eq_refl string.
+  Definition eq_sym := @eq_sym string.
+  Definition eq_trans := @eq_trans string.
+  Definition lt_trans := lt_string_trans.
+  Definition lt_not_eq := lt_string_not_eq.
+  Definition compare x y := compare_string x y.
+  Definition eq_dec := string_dec.
+End string_as_OT.
+
+Module reference_as_OT <: UsualOrderedType.
+  Definition t := reference.
+  Definition eq := @eq reference.
+  Definition lt := lt_reference.
+  Definition eq_refl := @eq_refl reference.
+  Definition eq_sym := @eq_sym reference.
+  Definition eq_trans := @eq_trans reference.
+  Definition lt_trans := lt_reference_trans.
+  Definition lt_not_eq := lt_reference_not_eq.
+  Definition compare (ref_variable xs xl) (ref_variable ys yl) :=
+    match (
+End reference_as_OT.
